Veritas.EAC.fst
@@ -1,0 +1,97 @@
+module Veritas.EAC
+
+open FStar.Seq
+open Veritas.Hash
+open Veritas.Interleave
+open Veritas.Key
+open Veritas.MultiSetHash
+open Veritas.Record
+open Veritas.SeqAux
+open Veritas.State
+open Veritas.Verifier
+
+//Allow the solver to unroll recursive functions at most once (fuel)
+//Allow the solver to invert inductive definitions at most once (ifuel)
+#push-options "--max_fuel 1 --max_ifuel 1 --initial_fuel 1 --initial_ifuel 1"
+
+type eac_state = 
+  | EACFail: eac_state  
+  | EACInit: eac_state
+  | EACInCache: m:add_method -> k:key -> v:value -> eac_state
+  | EACEvicted: m:add_method -> k:key -> v:value -> eac_state
+
+let eac_add (e: vlog_entry) (s: eac_state) : eac_state = 
+  match s with
+  | EACFail -> EACFail
+  | EACInit -> (
+    match e with 
+    | AddM (k,v) _ -> if v = init_value k then EACInCache MAdd k v
+                      else EACFail
+    | _ -> EACFail
+  )
+  
+  | EACInCache m k v -> (
+    match e with 
+    | Get k' v' -> if k' = k && (DVal v') = v then s
+                   else EACFail
+    | Put k' v' -> if k' = k then EACInCache m k (DVal v')
+                   else EACFail 
+    | EvictM k' _ -> if k' = k then EACEvicted MAdd k v
+                     else EACFail
+    | EvictBM k' _ _ -> if k' = k && m = MAdd then EACEvicted BAdd k v
+                        else EACFail
+    | EvictB k' _ -> if k' = k && m = BAdd then EACEvicted BAdd k v
+                     else EACFail
+    | _ -> EACFail
+  )
+  
+  | EACEvicted m k v -> (
+    match e with
+    | AddM (k',v') _ -> if k' = k && v' = v && m = MAdd then EACInCache MAdd k v
+                        else EACFail
+    | AddB (k',v') _ _ -> if k' = k && v' = v && m = BAdd then EACInCache BAdd k v
+                          else EACFail
+    | _ -> EACFail
+  )
+                                
+let eac_verify (l: vlog) = reduce EACInit eac_add l
+
+let vlog_entry_key (e: vlog_entry) = 
+  match e with
+  | Get k _ -> k
+  | Put k _ -> k
+  | AddM (k,_) _ -> k
+  | EvictM k _ -> k
+  | AddB (k,_) _ _ -> k
+  | EvictB k _ -> k
+  | EvictBM k _ _ -> k
+
+(* filter out entries of vlog affecting key k *)
+let key_vlog (k: key) (l: vlog) = filter (fun e -> k = vlog_entry_key e) l
+
+(* evict add consistency *)
+let eac (l:vlog) = forall (k: key). ~(EACFail? (eac_verify (key_vlog k l)))
+
+(* refinement of evict add consistent logs *)
+type eac_log = l:vlog{eac l}
+
+(* the state operations of a vlog *)
+let is_state_op (e: vlog_entry) = 
+  match e with
+  | Get k v -> true
+  | Put k v -> true 
+  | _ -> false
+
+(* map vlog entry to state op *)
+let to_state_op (e:vlog_entry {is_state_op e}) = 
+  match e with
+  | Get k v -> Veritas.State.Get k v
+  | Put k v -> Veritas.State.Put k v
+
+(* filter out the state ops of vlog *)
+let to_state_op_vlog (l: vlog) = 
+  map to_state_op (filter_refine is_state_op l)
+
+(* evict add consistency implies rw-consistency *)
+let lemma_eac_implies_rw_consistent (l:eac_log):
+  Lemma (rw_consistent (to_state_op_vlog l)) = admit()
